WIP proof for close of small filter

deps/poulet4/lib/P4automata/Benchmarks/SmallFilterProof.v
@@ -1,37 +1,239 @@
-Require Import Poulet4.P4automata.Examples.ProofHeader.
-Require Import Poulet4.P4automata.Examples.SmallFilter.
-From Hammer Require Import Tactics.
+Require Import Poulet4.P4automata.Benchmarks.ProofHeader.
+Require Import Poulet4.P4automata.Benchmarks.SmallFilter.
+
+Require Import Poulet4.P4automata.CompileConfRel.
+Require Import Poulet4.P4automata.FirstOrder.
+Require Import Poulet4.P4automata.FirstOrderConfRel.
+Require Import Poulet4.P4automata.CompileConfRelSimplified.
+Require Import Poulet4.P4automata.CompileFirstOrderConfRelSimplified.
+
+Require Import Poulet4.P4automata.WP.
+Require Import Coq.Program.Equality.
 
 
 Notation H := (IncrementalBits.header + BigBits.header).
 Notation A := IncrementalSeparate.aut.
 Notation conf := (P4automaton.configuration (P4A.interp A)).
+
 Definition r_states :=
-  Eval cbv in (Reachability.reachable_states IncrementalSeparate.aut 10 IncrementalBits.Start BigBits.Parse).
+  Eval vm_compute in (Reachability.reachable_states
+                        IncrementalSeparate.aut
+                        200
+                        IncrementalBits.Start
+                        BigBits.Parse).
+
+Definition top : Relations.rel conf := fun _ _ => True.
+
+
+Ltac extend_bisim :=
+  match goal with
+  | |- pre_bisimulation ?a ?wp ?i ?R (?C :: _) _ _ =>
+    let H := fresh "H" in
+    assert (H: ~interp_entailment A i ({| e_prem := R; e_concl := C |}));
+    [ idtac |
+    pose (t := WP.wp r_states C);
+    eapply PreBisimulationExtend with (H0 := right H) (W := t);
+    [ tauto | trivial |];
+    vm_compute in t;
+    simpl (_ ++ _);
+    clear t]
+  end.
+
+Ltac skip_bisim :=
+  match goal with
+  | |- pre_bisimulation ?a ?wp ?i ?R (?C :: _) _ _ =>
+    let H := fresh "H" in
+    assert (H: interp_entailment A i ({| e_prem := R; e_concl := C |}));
+    eapply PreBisimulationSkip with (H0:=left H);
+    [ exact I | ];
+    clear H
+  end.
+
+Ltac extend_bisim' HN :=
+  match goal with
+  | |- pre_bisimulation ?a _ _ _ (?C :: _) _ _ =>
+    pose (t := WP.wp r_states C);
+    eapply PreBisimulationExtend with (H0 := right HN) (W := t);
+    [ tauto | trivial |];
+    vm_compute in t;
+    simpl (_ ++ _);
+    clear t;
+    clear HN
+  end.
+
+Ltac skip_bisim' H :=
+  eapply PreBisimulationSkip with (H0:=left H);
+  [ exact I | ];
+  clear H.
+
+Ltac size_script :=
+  unfold Syntax.interp;
+  autorewrite with size';
+  vm_compute;
+  repeat constructor.
+
+
+Declare ML Module "mirrorsolve".
+
+RegisterPrim (@TVar (sig A) (CEmp _) (Bits 0)) "p4a.core.var".
+RegisterPrim (@TFun (sig A) (CEmp _) [] (Bits 0)) "p4a.core.fun".
+
+RegisterPrim (@VHere (sig A) (CEmp _) (Bits 0)) "p4a.core.vhere".
+RegisterPrim (@VThere (sig A) (CEmp _) (Bits 0) (Bits 0)) "p4a.core.vthere".
+
+
+RegisterPrim (@FEq (sig A) (CEmp _) (Bits 0)) "p4a.core.eq".
+RegisterPrim (@FTrue (sig A) (CEmp _)) "p4a.core.tt".
+RegisterPrim (@FFalse (sig A) (CEmp _)) "p4a.core.ff".
+RegisterPrim (@FRel (sig A) (CEmp _)) "p4a.core.rel".
+RegisterPrim (@FNeg (sig A) (CEmp _)) "p4a.core.neg".
+RegisterPrim (@FOr (sig A) (CEmp _)) "p4a.core.or".
+RegisterPrim (@FAnd (sig A) (CEmp _)) "p4a.core.and".
+RegisterPrim (@FForall (sig A) (CEmp _)) "p4a.core.forall".
+
+RegisterPrim (@FImpl (sig A) (CEmp _)) "p4a.core.impl".
+
+RegisterPrim (@CEmp (sig A)) "p4a.core.cnil".
+RegisterPrim (@CSnoc (sig A)) "p4a.core.csnoc".
+
+RegisterPrim (@inl nat bool) "coq.core.inl".
+RegisterPrim (@inr nat bool) "coq.core.inr".
+
+
+RegisterPrim FirstOrderConfRelSimplified.Bits "p4a.sorts.bits".
+RegisterPrim FirstOrderConfRelSimplified.Store "p4a.sorts.store".
+
+RegisterPrim FirstOrderConfRelSimplified.BitsLit "p4a.funs.bitslit".
+RegisterPrim FirstOrderConfRelSimplified.Concat "p4a.funs.concat".
+RegisterPrim FirstOrderConfRelSimplified.Slice "p4a.funs.slice".
+RegisterPrim FirstOrderConfRelSimplified.Lookup "p4a.funs.lookup".
+
+RegisterPrim (@HList.HNil nat (fun _ => bool)) "p4a.core.hnil".
+RegisterPrim (@HList.HCons nat (fun _ => bool)) "p4a.core.hcons".
+
+RegisterEnvCtors (IncrementalBits.Pref, FirstOrderConfRelSimplified.Bits 1)  (IncrementalBits.Suf, FirstOrderConfRelSimplified.Bits 1) (BigBits.Pref, FirstOrderConfRelSimplified.Bits 1) (BigBits.Suf, FirstOrderConfRelSimplified.Bits 1).
+
+Ltac crunch_foterm :=
+  match goal with
+  | |- interp_fm _ ?g =>
+    let temp := fresh "temp" in set (temp := g);
+    vm_compute in temp;
+    subst temp
+  end.
+
+Ltac verify_interp :=
+  match goal with
+  | |- pre_bisimulation ?a ?wp _ ?R (?C :: _) _ _ =>
+    let H := fresh "H" in
+    assert (H: interp_entailment A top ({| e_prem := R; e_concl := C |}));
+    [
+      eapply simplify_entailment_correct with (i := fun _ _ => True);
+      eapply compile_simplified_entailment_correct;
+      [ typeclasses eauto | typeclasses eauto | ];
+
+      time "reduce goal" crunch_foterm;
+
+      match goal with
+      | |- ?X => time "smt check neg" check_interp_neg X
+      | |- ?X => time "smt check pos" check_interp_pos X; admit
+      end
+    |]
+  end;
+  let n:= numgoals in
+  tryif ( guard n = 2) then
+    match goal with
+    | |- interp_fm _ _ => admit
+    | H : interp_entailment _ _ _ |- pre_bisimulation _ _ _ ?R (?C :: _) _ _ =>
+      clear H;
+      let HN := fresh "HN" in
+      assert (HN: ~ (interp_entailment A top ({| e_prem := R; e_concl := C |}))) by admit
+    end
+  else idtac.
+
+Ltac run_bisim :=
+  verify_interp;
+  match goal with
+  | HN: ~ (interp_entailment _ _ _ ) |- _ =>
+    idtac "extending"; extend_bisim' HN; clear HN
+  | H: interp_entailment _ _ _  |- _ =>
+    idtac "skipping"; skip_bisim' H; clear H
+  end.
+
+Require Import Poulet4.Relations.
+
+Lemma simplify_crel_correct':
+  forall i crs q1 q2,
+    ((i (conf_to_state_template q1) (conf_to_state_template q2) /\
+      interp_simplified_crel (List.map (simplify_conf_rel (a := A)) crs)
+                             q1.(conf_buf)
+                             q2.(conf_buf)
+                             q1.(conf_store)
+                             q2.(conf_store)) ->
+                             
+      interp_crel A (fun c1 c2 => i (conf_to_state_template c1) (conf_to_state_template c2)) crs q1 q2
+     ).
+  Proof.
+  Admitted.
+
 
 Lemma prebisim_incremental_sep:
-  pre_bisimulation IncrementalSeparate.aut
-                   (WPSymLeap.wp r_states (H:=IncrementalSeparate.header))
-                   (Reachability.reachable_pair r_states)
-                   nil
-                   (mk_init _ _ _ IncrementalSeparate.aut 10 IncrementalBits.Start BigBits.Parse)
-                   (inl (inl IncrementalBits.Start), [], [])
-                   (inl (inr BigBits.Parse), [], []).
+  pre_bisimulation A
+                   (wp r_states)
+                   top
+                   []
+                   (mk_init _ _ _ A 10 IncrementalBits.Start BigBits.Parse)
+                   (P4automaton.MkConfiguration
+                    (Syntax.interp A)
+                    (inl (inl IncrementalBits.Start))
+                    0
+                    tt
+                    ltac:(eapply cap')
+                    nil)
+                    (P4automaton.MkConfiguration
+                      (Syntax.interp A)
+                      (inl (inr BigBits.Parse))
+                      0
+                      tt
+                      ltac:(eapply cap')
+                      nil).
 Proof.
-  set (r := (mk_init _ _ _ IncrementalSeparate.aut 10 IncrementalBits.Start BigBits.Parse)).
-  cbv in r.
-  subst r.
-  solve_bisim.
-  solve_bisim.
-  solve_bisim.
-  solve_bisim.
-  solve_bisim.
-  solve_bisim.
-  solve_bisim.
-  cbv.
-  sauto.
-  Unshelve.
-  exact nil.
-  exact nil.
-  exact nil.
-Qed.
+  set (rel0 := (mk_init _ _ _ A 10 IncrementalBits.Start BigBits.Parse)).
+  cbv in rel0.
+  subst rel0.
+  time "overall loop" (repeat time "bisim step" run_bisim).
+
+  match goal with 
+  | |- pre_bisimulation _ _ _ ?R _ _ _ => 
+    set (temp := R)
+  end.
+
+  set (tempA := A).
+
+  apply PreBisimulationClose with (a := tempA).
+
+  Opaque interp_crel.
+
+  match goal with 
+  | |- interp_crel _ _ _ ?Q1 ?Q2 => 
+    set (q1 := Q1); set (q2 := Q2)
+  end.
+
+  pose proof simplify_crel_correct'.
+
+
+  specialize (H (fun _ _ => True) temp q1 q2).
+  eapply H. split; trivial.
+
+
+  eapply compile_crel_correct; [typeclasses eauto | typeclasses eauto|].
+
+  eapply quantify_all_correct.
+
+  crunch_foterm.
+
+  (* huh... *)
+  try match goal with
+  | |- ?X => time "smt check pos" check_interp_pos X
+  end.
+
+Admitted.
